\documentclass{article}
\usepackage[utf8]{inputenc}
\usepackage{amsmath}
\linespread{1.5}
\title{Advanced Digital Signal Processing Exams}
\author{CHEN SHANG }
\date{Nov 2022}

\begin{document}

\maketitle
{\Huge
Personal answers.\par
May not always be right.\par}
\section*{2018-2019}
\subsection*{1.}
\subsubsection*{(a)}
\subsubsection*{(b)}

\subsection*{2.}
\subsubsection*{(a)}
(i)\par
(ii)\par
\subsubsection*{(b)}

\subsection*{3.}
\subsubsection*{(a)}
\subsubsection*{(b)}
\subsubsection*{(c)}

\subsection*{4.}
\subsubsection*{(a)}
\subsubsection*{(b)}
\subsubsection*{(c)}

\subsection*{5.}
\subsubsection*{(a)}
\subsubsection*{(b)}
\subsubsection*{(c)}
\clearpage

\section*{2019-2020}
\subsection*{1.}
\subsubsection*{(a)}
\subsubsection*{(b)}
$\uparrow 5 \ \downarrow 5 \ \downarrow 3 \ \uparrow 3$\par
$\downarrow 3 \ \uparrow 3$\par
$y(n)=\begin{cases}
x(n) \ & n=0,\pm 3,\pm6...\\
0 \ &{\rm otherwise}
\end{cases}$
\subsection*{2.}
\subsubsection*{(a)}
$V(z)=\frac{1}{D}\sum_{k=0}^{D-1}H_{D}(e^{-j2\pi\frac{ k}{D}}z^{\frac{1}{D}})X(e^{-j2\pi\frac{ k}{D}}z^{\frac{1}{D}})=\frac{1}{2}[X(z^{\frac{1}{2}})+X(-z^{\frac{1}{2}})]$\par
$W(z)=\frac{1}{2}z^{-\frac{1}{2}}[X(z^{\frac{1}{2}})-X(-z^{\frac{1}{2}})]$\par
$V_{n}(z)=\frac{1}{2}[X(z)+X(-z)]$\par
$W_{n}(z)=\frac{1}{2}z^{-1}[X(z)-X(-z)]$\par
$Y(z)=W_{n}(z)+z^{-1}V_{n}(z)$\par
\subsubsection*{(b)}
(i)\par
$F_{SC}=100$\par
$D=\frac{F}{2F_{SC}}=50$\par
$\Delta f=\frac{f_{s}-f_{p}}{F}=\frac{65-60}{10\times 10^3}$\par
$M=\frac{-10{\rm log}_{10}\delta_{s}\delta_{p}-13}{14.6\Delta f}+1=5000$\par
???
(ii)\par

\subsection*{3.}
\subsubsection*{(a)}
(i)\par
(ii)\par
(iii)\par
\subsubsection*{(b)}
$\begin{bmatrix}
H_{0}(z)\\
H_{1}(z)\\
H_{2}(z)\\
\end{bmatrix}=\begin{bmatrix}
4 &6 &1\\
2 &1 &0\\
1 &0 &0\\
\end{bmatrix}\begin{bmatrix}
1\\
z^{-1}\\
z^{-2}\\
\end{bmatrix}$\par\indent
\par\indent\par
$P(z)=\begin{bmatrix}
4 &6 &1\\
2 &1 &0\\
1 &0 &0\\
\end{bmatrix}$\par\indent
\par\indent
\par
$Q(z)=P^{-1}(z)=\begin{bmatrix}
0 &0 &1\\
0 &1 &-2\\
1 &-6 &8\\
\end{bmatrix}$\par\indent
\par\indent
\par
$G(z)=\begin{bmatrix}
G_{0}(z)\\
G_{1}(z)\\
G_{2}(z)\\
\end{bmatrix}=z^{-2}\begin{bmatrix}
0 &0 &1\\
0 &1 &-2\\
1 &-6 &8\\
\end{bmatrix}\begin{bmatrix}
1\\
z^{-1}\\
z^{-2}\\
\end{bmatrix}=\begin{bmatrix}
1\\
z^{-1}-2\\
z^{-2}-6z^{-1}+8\\
\end{bmatrix}$\par

\subsection*{4.}
\subsubsection*{(a)}
\subsubsection*{(b)}
\subsubsection*{(c)}
\subsubsection*{(d)}

\subsection*{5.}
\subsubsection*{(a)}
\subsubsection*{(b)}

\clearpage


\section*{2020-2021}
\subsection*{1.}
\subsubsection*{(a)}
(i)\par
(ii)\par
\subsubsection*{(b)}

\subsection*{2.}
\subsubsection*{(a)}
\subsubsection*{(b)}


\subsection*{3.}
\subsubsection*{(a)}
\subsubsection*{(b)}


\subsection*{4.}
\subsubsection*{(a)}
\subsubsection*{(b)}
(i)\par
(ii)\par
(iii)\par


\clearpage






\section*{2021-2022}
\subsection*{1.}
\subsubsection*{(a)}
(i)\par
$x(n)=x_{a}(nT_{s})=x_{a}(\frac{n}{20})=2cos(\frac{3\pi n}{10})+sin(\frac{3\pi n}{5})$\par
(ii)\par
$V(z)=\frac{1}{D}\sum_{k=0}^{D-1}X(z^{\frac{1}{D}}e^{-j\frac{2\pi k}{D}})=\frac{1}{2}[X(z^{\frac{1}{2}})+X(-z^{\frac{1}{2}})]$\par
$z=e^{j\omega}$\par
$V(\omega)=\frac{1}{2}[X(e^{j\frac{\omega}{2}})+X(e^{j(\frac{\omega}{2}-\pi)})]=\frac{1}{2}[X(\frac{\omega}{2})+X(\frac{\omega}{2}-\pi)]$\par
(iii)\par
(iv)\par
???
\subsubsection*{(b)}
(i)\par
$\Delta f=\frac{f_{s}-f_{p}}{F}$\par
$N=\frac{-10{\rm log}_{10}\delta_{s}\delta_{p}-13}{14.6\Delta f}+1=762$\par
$762\div 6=127$\par
(ii)\par
Week7 \ 41:16


\subsection*{2.}
\subsubsection*{(a)}
(i)\par
$V=X+\beta V z^{-2}$\par
$Y=\alpha V+Vz^{-1}+Vz^{-2}$\par
$\frac{V}{X}=\frac{1}{1-\beta z^{-2}}$\par
$\frac{Y}{V}=\alpha +z^{-1}+z^{-2}$\par
$P(z)=\frac{Y}{X}=\frac{\alpha +z^{-1}+z^{-2}}{1-\beta z^{-2}}$\par
(ii)\par
$P(z)=\frac{Y}{X}=\frac{(1-\frac{1}{2} z^{-1})(\alpha-2z^{-1})}{(1-\frac{1}{2} z^{-1})(1+\frac{1}{2} z^{-1})}$\par
$P(z)=\frac{Y}{X}=\frac{(1+\frac{1}{2} z^{-1})(\alpha+2z^{-1})}{(1-\frac{1}{2} z^{-1})(1+\frac{1}{2} z^{-1})}$\par
$\alpha=-2 \quad {\rm or} \quad \alpha=-6$\par
(iii)\par
$P(z)=2+z^{-1}+z^{-2}$\par
$Q(z)=z^{-2}P(z^{-1})=1+z^{-1}+2z^{-2}$\par
$H(z)=P(z)Q(z)$\par
$H(\omega)=e^{-j2\omega}(6+6cos\omega+4cos2\omega)$\par
$e^{-j2\omega}$ is the phase of $H(\omega)$\par
\subsubsection*{(b)}
(i)\par
$V_{1}(z)=V(z^4)$\par
$V_{2}(z)=V_{1}(z)R(z)$\par
$V_{3}(z)=z^{-1}V_{2}(z)$\par
$W(z)=\frac{1}{4}\sum_{k=0}^{3}V_{3}(e^{-j2\pi \frac{k}{4}}z^{\frac{1}{4}})$\par
$H(z)=\frac{W(z)}{V(z)}$\par
Due to downsampling operation, this system is not time-invariant.\par
(ii)\par
???
\subsection*{3.}
\subsubsection*{(a)}
(i)\par
(ii)\par
(iii)\par
\subsubsection*{(b)}
(i)\par
(ii)\par

\subsection*{4.}
\subsubsection*{(a)}
(i)\par
(ii)\par
\subsubsection*{(b)}
(i)\par
$H_{1}(z)=1-z^{-2}$\par
$\Gamma_{h_{1}h_{1}}(f)=H_{1}(z)H_{1}(z^{-1})|_{z=e^{j2\pi f}}=2-z^{2}-z^{-2}$\par
$\Gamma_{ww}(f)=\sigma_{w}^2$\par
$\Gamma_{xx}(f)=\Gamma_{h_{1}h_{1}}(f)\Gamma_{ww}(f)=\sigma_{w}^2(2-z^{2}-z^{-2})$\par
$H_{2}(z)=\frac{1}{1+0.81z^{-2}}$\par
$\Gamma_{h_{2}h_{2}}(f)=H_{2}(z)H_{2}(z^{-1})|_{z=e^{j2\pi f}}=\frac{1}{1.6561+0.81z^{2}+0.81z^{-2}}$\par
$\Gamma_{yy}(f)=\Gamma_{h_{2}h_{2}}(f)\Gamma_{ww}(f)=\frac{\sigma_{w}^2}{1.6561+0.81z^{2}+0.81z^{-2}}$\par
(ii)\par
(iii)\par
$\Gamma_{yy}(f)=\frac{\sigma_{w}^2}{1.6561+0.81z^{2}+0.81z^{-2}}=\sigma_{w}^2\frac{z^{2}}{0.81z^{4}+1.6561z^{2}+0.81}$\par

\subsection*{5.}
\subsubsection*{(a)}
$A_{2}(z)=1+2z^{-1}+\frac{1}{3}z^{-2}$\par
$K_{2}=\frac{1}{3}$\par
$B_{2}(z)=\frac{1}{3}+2z^{-1}+z^{-2}$\par
$A_{1}(z)=\frac{A_{2}(z)-K_{2}B_{2}(z)}{1-K_{2}^{2}}=1+\frac{3}{2}z^{-1}$\par
$K_{1}=\frac{3}{2}$\par
\subsubsection*{(b)}
$H_{sv}(z)=\frac{1}{1-0.8z^{-1}}$\par
$\Gamma_{ss}(\omega)=\sigma_{v}^{2}H_{sv}(\omega)H_{sv}(-\omega)$\par
12.14
\clearpage

\end{document}
